LeanLambdaLibMathlib/LambdaLib/unificationFacts.lean
@@ -1,0 +1,248 @@
+import LambdaLib.qterm
+
+open QuotTerm
+
+theorem lam_body_rw {t1 t2 s1 s2} : (lam s1 t1 = lam s2 t2) = (t1 = t2) := by
+  apply propext
+  apply Iff.intro
+  · apply lam_body
+  · intros
+    subst_vars
+    exact alpha
+
+theorem const_inj_rw {c1 c2} : (const c1 = const c2) = (c1 = c2) := by
+  apply propext
+  apply Iff.intro
+  · apply const_inj
+  · intros; subst_vars; rfl
+
+theorem var_inj_rw {i1 i2} : (var i1 = var i2) = (i1 = i2) := by
+  apply propext
+  apply Iff.intro
+  · apply var_inj
+  · intros; subst_vars; rfl
+
+theorem var_not_const_rw {i c} : (var i = const c) = False := by
+  apply propext
+  apply Iff.intro
+  · apply var_not_const
+  · intros; contradiction
+
+theorem var_not_const_rw2 {i c} : (const c = var i) = False := by
+  rw (config := {occs := .pos [2]}) [propext (Iff.intro Eq.symm Eq.symm)]
+  apply var_not_const_rw
+
+open SynTerm
+
+inductive Neutral : Term → Prop where
+| const : ∀{c}, Neutral (Term.const c)
+| var : ∀{n}, Neutral (Term.var n)
+| app : ∀{t arg}, Neutral t → Neutral (Term.app t arg)
+
+theorem stepNeutral {t1 t2} (step : (union Step StepEta) t1 t2)
+  (H : Neutral t1)
+  : Neutral t2 := by
+  cases step with
+  | r step => cases step with
+    | app1 step =>
+      cases H
+      constructor
+      apply (stepNeutral (union.r step))
+      assumption
+    | app2 _ =>
+      cases H
+      constructor
+      assumption
+    | beta =>
+      cases H with | app H => _
+      cases H
+    | lam _ => cases H
+  | s step => cases step with
+    | app1 step =>
+      cases H
+      constructor
+      apply (stepNeutral (union.s step))
+      assumption
+    | app2 _ =>
+      cases H
+      constructor
+      assumption
+    | _ => cases H
+
+theorem allstepNeutral {t1 t2} (step : AllStep t1 t2)
+  (H : Neutral t1)
+  : Neutral t2 := by
+  induction step with
+  | refl => assumption
+  | cons _ _ ih =>
+    apply ih
+    apply stepNeutral <;> assumption
+
+def SmallStep := closeRef (union Step StepEta)
+
+lemma appStep' {a b t} (step : (union Step StepEta) (Term.app a b) t) (neut : Neutral a)
+  : ∃ a' b', t = Term.app a' b' ∧ SmallStep a a' ∧ SmallStep b b' /-Neutral a'-/ := by
+  cases step with | r step => _ | s step => _ <;> cases step <;> (try (cases neut; done))
+  · refine ⟨_, _, rfl, ?_⟩
+    apply And.intro
+    · apply Or.inr
+      apply union.r
+      assumption
+    · apply Or.inl
+      rfl
+  · refine ⟨_, _, rfl, ?_⟩
+    apply And.intro
+    · apply Or.inl
+      rfl
+    · apply Or.inr
+      apply union.r
+      assumption
+  · refine ⟨_, _, rfl, ?_⟩
+    apply And.intro
+    · apply Or.inr
+      apply union.s
+      assumption
+    · apply Or.inl
+      rfl
+  · refine ⟨_, _, rfl, ?_⟩
+    apply And.intro
+    · apply Or.inl
+      rfl
+    · apply Or.inr
+      apply union.s
+      assumption
+
+theorem appStep {a b t} (step : AllStep (Term.app a b) t) (neut : Neutral a)
+  : ∃ a' b', t = Term.app a' b' ∧ AllStep a a' ∧ AllStep b b' := by
+  generalize eqn : (Term.app a b) = t1 at *
+  induction step generalizing a b with
+  | refl =>
+    subst_vars
+    exists a, b
+    exact ⟨rfl, closure.refl, closure.refl⟩
+  | cons s ss ih =>
+    subst_vars
+    have ⟨a', b', eq, stepa, stepb⟩ := appStep' s neut
+    have neut' := allstepNeutral (closeRefToClosure stepa) neut
+    subst_vars
+    -- have test := (ih neut' rfl)
+    have ⟨ a'', b'', eq, ssa, ssb⟩  := ih neut' rfl
+    subst_vars
+    exists a'', b''
+    apply And.intro
+    · rfl
+    · apply And.intro
+      · exact (transitivity (closeRefToClosure stepa) ssa)
+      · exact (transitivity (closeRefToClosure stepb) ssb)
+
+inductive QNeutral : QTerm → Prop where
+| const : ∀{c}, QNeutral (const c)
+| var : ∀{n}, QNeutral (var n)
+| app : ∀{t arg}, QNeutral t → QNeutral (app t arg)
+
+theorem liftNeutralWithArity {t}
+  : Neutral t → QNeutral (Quotient.mk _ t) := by
+  intro H
+  induction H with
+  | @const c =>
+    have thing := @QNeutral.const c
+    unfold const at thing
+    assumption
+  | @var i =>
+    have thing := @QNeutral.var i
+    unfold var at thing
+    assumption
+  | @app a b qn =>
+    -- apply Quotient.ind _ a
+    have thing := @QNeutral.app ⟦a⟧ ⟦b⟧
+    simp [app] at thing
+    apply thing
+    assumption
+
+theorem lowerNeutralWithArity {q} (H : QNeutral q)
+  : ∃ t, ⟦t⟧ = q ∧ Neutral t := by
+  induction H with
+  | @const c =>
+    exists .const c
+    simp [const]
+    repeat' constructor
+  | @var i =>
+    exists .var i
+    simp [var]
+    repeat' constructor
+  | @app a b qn ih =>
+    rcases ih with ⟨t, rfl, neu⟩
+    apply Quotient.ind _ b
+    intro b
+    exists .app t b
+    simp [app]
+    constructor
+    assumption
+
+theorem app_ne_var {i a b} (qneut : QNeutral a) (eq : var i = app a b) : False := by
+  have ⟨t, eq2, neut⟩ := lowerNeutralWithArity qneut
+  subst_vars
+  revert eq
+  apply Quotient.ind _ b
+  intro b eq
+  simp [var, app] at eq
+  have ⟨t', l, r⟩ := Quotient.exact eq
+  rcases varStep l with rfl
+  rcases appStep r neut with ⟨_, _, eq⟩
+  rcases eq with ⟨eq, _, _⟩
+  cases eq
+
+theorem app_ne_const {c a b} (qneut : QNeutral a) (eq : const c = app a b) : False := by
+  have ⟨t, eq2, neut⟩ := lowerNeutralWithArity qneut
+  subst_vars
+  revert eq
+  apply Quotient.ind _ b
+  intro b eq
+  simp [const, app] at eq
+  have ⟨t', l, r⟩ := Quotient.exact eq
+  rcases constStep l with rfl
+  rcases appStep r neut with ⟨_, _, eq⟩
+  rcases eq with ⟨eq, _, _⟩
+  cases eq
+
+theorem app_fact {a b a' b'} (qneut : QNeutral a) (qneut' : QNeutral a')
+  (eq : app a b = app a' b') : a = a' /\ b = b' := by
+  have ⟨t, eq2, neut⟩ := lowerNeutralWithArity qneut
+  have ⟨t, eq2, neut'⟩ := lowerNeutralWithArity qneut'
+  subst_vars
+  revert eq
+  apply Quotient.ind _ b
+  apply Quotient.ind _ b'
+  intro b b' eq
+  simp [app] at eq
+  have ⟨t', l, r⟩ := Quotient.exact eq
+  rcases appStep l neut with ⟨_, _, eq, x, y⟩
+  rcases appStep r neut' with ⟨_, _, eq, z, w⟩
+  subst_vars
+  cases eq
+  apply And.intro <;> apply Quotient.sound
+  · refine ⟨_, x, z⟩
+  · refine ⟨_, y, w⟩
+
+theorem app_ne_var_rw {i a b} (qneut : QNeutral a) : (var i = app a b) = False := by
+  apply propext
+  apply Iff.intro
+  · apply app_ne_var qneut
+  · intros
+    contradiction
+
+theorem app_ne_const_rw {c a b} (qneut : QNeutral a) : (const c = app a b) = False := by
+  apply propext
+  apply Iff.intro
+  · apply app_ne_const qneut
+  · intros
+    contradiction
+
+theorem app_fact_rw {a b a' b'} (qneut : QNeutral a) (qneut' : QNeutral a')
+  : (app a b = app a' b') = (a = a' /\ b = b') := by
+  apply propext
+  apply Iff.intro
+  · apply app_fact qneut qneut'
+  · intro ⟨eq1, eq2⟩
+    subst_vars
+    rfl
